Moving more theorems around
Mostly out of typeSoundScript and into typeSysPropsScript or
weakeningScript, as made sense.

metatheory/typeSysPropsScript.sml
@@ -13,6 +13,10 @@ val find_recfun_def = semanticPrimitivesTheory.find_recfun_def;
 val same_tid_def = semanticPrimitivesTheory.same_tid_def;
 val lookup_con_id_def = semanticPrimitivesTheory.lookup_con_id_def;
 val merge_envC_def = semanticPrimitivesTheory.merge_envC_def;
+val lookup_var_id_def = semanticPrimitivesTheory.lookup_var_id_def;
+
+val type_env_cases = List.nth (CONJUNCTS type_v_cases, 2);
+val consistent_mod_cases = List.nth (CONJUNCTS type_v_cases, 3);
 
 (* ---------- check_freevars ---------- *)
 
@@ -340,6 +344,25 @@ rw [deBruijn_subst_def, LENGTH_COUNT_LIST, EL_MAP, EL_COUNT_LIST,
     check_freevars_def] >>
 metis_tac []);
 
+val type_subst_lem1 = 
+(GEN_ALL o
+ SIMP_RULE (srw_ss()++ARITH_ss) [] o
+ Q.SPECL [`[]`, `t`, `0`, `targs`, `tvs`] o
+ SIMP_RULE (srw_ss()) [GSYM RIGHT_FORALL_IMP_THM])
+check_freevars_subst_inc
+
+val type_subst_lem3 = Q.prove (
+`!skip targs t tvs.
+  (skip = 0) ∧
+  EVERY (check_freevars tvs []) targs ∧
+  check_freevars (LENGTH targs) [] t 
+  ⇒
+  check_freevars tvs [] (deBruijn_subst skip targs t)`,
+ho_match_mp_tac deBruijn_subst_ind >>
+rw [check_freevars_def, deBruijn_subst_def, EVERY_MAP] >>
+fs [EVERY_MEM, MEM_EL] >>
+metis_tac []);
+
 (* ---------- tenvC stuff ----------*)
 (* merge_tenvC, lookup_con_id, flat_tenvC_ok, tenvC_ok *)
 
@@ -421,6 +444,33 @@ val tenvC_ok_lookup = Q.store_thm ("tenvC_ok_lookup",
  fs [] >>
  imp_res_tac flat_tenvC_ok_lookup >>
  fs [EVERY_MEM]);
+
+val merge_tenvC_empty_assoc = Q.store_thm ("merge_tenvC_empty_assoc",
+`!tenvC1 tenvC2 tenvC3.
+  merge_tenvC ([],tenvC1) (merge_tenvC ([],tenvC2) tenvC3)
+  =
+  merge_tenvC ([],tenvC1++tenvC2) tenvC3`,
+ rw [] >>
+ PairCases_on `tenvC3` >>
+ rw [merge_tenvC_def, merge_def]);
+
+val merge_envC_empty = Q.store_thm ("merge_envC_empty",
+`(!envC. merge_envC ([],[]) envC = envC) ∧
+ (!tenvC. merge_tenvC ([],[]) tenvC = tenvC)`,
+ rw [] >>
+ TRY (PairCases_on `envC`) >>
+ TRY (PairCases_on `tenvC`) >>
+ rw [merge_envC_def, merge_tenvC_def, merge_def]);
+
+val lookup_con_id_mod_cons = Q.store_thm ("lookup_con_id_mod_cons",
+`!mn cn mn' flat_envC1 envC1 flat_envC2.
+  lookup_con_id (Long mn cn) ((mn',flat_envC1)::envC1,flat_envC2) =
+  if mn = mn' then
+    lookup cn flat_envC1
+  else
+    lookup_con_id (Long mn cn) (envC1,flat_envC2)`,
+rw [lookup_con_id_def]);
+
 
 (* ---------- tenv stuff ---------- *)
 (* bind_tvar, bind_var_list, bind_var_list2, lookup_tenv, bind_tenv,
@@ -679,6 +729,19 @@ val bvl2_to_bvl = Q.store_thm ("bvl2_to_bvl",
 ho_match_mp_tac bind_var_list_ind >>
 rw [bind_var_list_def, bind_var_list2_def, tenv_add_tvs_def]);
 
+val type_lookup_lem4 = Q.prove (
+`!tvs l tenv n t.
+  tenv_ok tenv ∧
+  (num_tvs tenv = 0) ∧
+  (lookup_tenv n 0 tenv = SOME (l,t))
+  ⇒
+  (lookup_tenv n tvs tenv = SOME (l,t))`,
+induct_on `tenv` >>
+rw [lookup_tenv_def, num_tvs_def, tenv_ok_def] >-
+metis_tac [] >>
+fs [] >>
+metis_tac [nil_deBruijn_inc]);
+
 (* ---------- tenvM stuff ---------- *)
 
 val tenvM_ok_lookup = Q.store_thm ("tenvM_ok_lookup",
@@ -724,6 +787,15 @@ fs [] >|
      imp_res_tac lookup_freevars >>
      `num_tvs tenv + tvs ≥ tvs` by decide_tac >>
      metis_tac [check_freevars_add]]);
+
+val tenvM_ok_pres = Q.store_thm ("tenvM_ok_pres",
+`∀tenvM mn tenv. 
+ tenvM_ok tenvM ∧
+ tenv_ok (bind_var_list2 tenv Empty)
+ ⇒
+ tenvM_ok (bind mn tenv tenvM)`,
+induct_on `tenvM` >>
+rw [tenvM_ok_def, bind_def]);
 
 (* ---------- type_uop ---------- *)
 
@@ -1334,6 +1406,41 @@ cases_on `tvs = 0` >>
 fs [check_freevars_def, num_tvs_bind_var_list, bind_tvar_def, num_tvs_def] >>
 metis_tac [arithmeticTheory.ADD_0]);
 
+val type_e_subst_lem = Q.prove (
+`(∀tenvM tenvC tenv e t targs tvs targs'.
+  type_e tenvM tenvC (bind_tenv x 0 t1 (bind_tvar (LENGTH targs) tenv)) e t ∧
+  (num_tvs tenv = 0) ∧ 
+  tenvM_ok tenvM ∧ 
+  tenvC_ok tenvC ∧ 
+  tenv_ok (bind_tvar (LENGTH targs) tenv) ∧
+  EVERY (check_freevars tvs []) targs ∧
+  check_freevars (LENGTH targs) [] t1
+  ⇒
+  type_e tenvM tenvC (bind_tenv x 0 (deBruijn_subst 0 targs t1) (bind_tvar tvs tenv)) e (deBruijn_subst 0 targs t))`,
+rw [bind_tenv_def] >>
+match_mp_tac ((SIMP_RULE (srw_ss()) [bind_tenv_def, num_tvs_def, deBruijn_subst_tenvE_def, db_merge_def, deBruijn_inc0] o
+               Q.SPECL [`tenvM`, `tenvC`, `e`, `t`, `bind_tenv x 0 t1 Empty`] o
+               SIMP_RULE (srw_ss()) [GSYM RIGHT_FORALL_IMP_THM, AND_IMP_INTRO] o
+               hd o
+               CONJUNCTS)
+              type_e_subst) >>
+rw [tenv_ok_def, bind_tvar_def, num_tvs_def] >>
+metis_tac []);
+
+val type_funs_subst_lem = 
+(Q.GEN `tenvE2` o
+ SIMP_RULE (srw_ss()) [bind_tenv_def, num_tvs_def, deBruijn_subst_tenvE_def,
+                       db_merge_def, deBruijn_inc0, num_tvs_bind_var_list,
+                       db_merge_bind_var_list,
+                       deBruijn_subst_E_bind_var_list] o
+ Q.SPECL [`tenvM`, `tenvC`, `e`, `t`, `bind_var_list 0 tenv' Empty`] o
+ SIMP_RULE (srw_ss()) [GSYM RIGHT_FORALL_IMP_THM, AND_IMP_INTRO] o
+ hd o
+ tl o
+ tl o
+ CONJUNCTS)
+type_e_subst;
+
 (* ---------- tid_exn_to_tc ---------- *)
 
 val tid_exn_to_tc_11 = Q.store_thm ("tid_exn_to_tc_11",
@@ -1345,6 +1452,13 @@ rw [tid_exn_to_tc_def, same_tid_def]);
 (* ---------- ctMap stuff ---------- *)
 (* flat_tenvC_ok, ctMap_ok, flat_to_ctMap_list, to_ctMap_list, flat_to_ctMap,
  * to_ctMap, ctMap_to_mods, tenvC_to_types *)
+
+val empty_to_ctMap = Q.store_thm ("empty_to_ctMap",
+`(!ctMap. FUNION (flat_to_ctMap []) ctMap = ctMap) ∧
+ (!ctMap. DISJOINT (FDOM (flat_to_ctMap [])) (FDOM ctMap))`,
+ rw [flat_to_ctMap_def, flat_to_ctMap_list_def, fmap_eq_flookup,
+     FLOOKUP_FUNION, flookup_fupdate_list, DISJOINT_DEF, EXTENSION,
+     FDOM_FUPDATE_LIST]);
 
 val ctMap_ok_merge_imp = Q.store_thm ("ctMap_ok_merge_imp",
 `!tenvC1 tenvC2.
@@ -1583,6 +1697,25 @@ val ctMap_ok_tenvC_ok = Q.store_thm ("ctMap_ok_tenvC_ok",
  res_tac >>
  fs []);
 
+val flat_to_ctMap_append = Q.store_thm ("flat_to_ctMap_append",
+`!tenvC1 tenvC2.
+  flat_to_ctMap (tenvC1++tenvC2) = FUNION (flat_to_ctMap tenvC1) (flat_to_ctMap tenvC2)`,
+rw [REVERSE_APPEND, flat_to_ctMap_def, flat_to_ctMap_list_def, fmap_eq_flookup,
+    flookup_fupdate_list, FLOOKUP_FUNION] >>
+every_case_tac >>
+fs [ALOOKUP_APPEND] >>
+every_case_tac >>
+fs []);
+
+val ctMap_to_mods_append = Q.store_thm ("ctMap_to_mods_append",
+`!ctMap1 ctMap2. ctMap_to_mods (FUNION ctMap1 ctMap2) = ctMap_to_mods ctMap1 ∪ ctMap_to_mods ctMap2`,
+ rw [ctMap_to_mods_def, EXTENSION] >>
+ metis_tac []);
+
+val to_ctMap_one_mod = Q.store_thm ("to_ctMap_one_mod",
+`!mn tenvC. to_ctMap ([(mn, tenvC)], emp) = flat_to_ctMap tenvC`,
+ rw [to_ctMap_def, to_ctMap_list_def, flat_to_ctMap_def, emp_def, flat_to_ctMap_list_def]);
+
 (* ---------- type_v, type_vs, type_env, consistent_mod_env ---------- *)
 
 val type_v_freevars = Q.store_thm ("type_v_freevars",
@@ -1614,6 +1747,283 @@ val type_v_freevars = Q.store_thm ("type_v_freevars",
                 arithmeticTheory.ADD, arithmeticTheory.ADD_COMM])
  >- metis_tac [check_freevars_add, arithmeticTheory.ZERO_LESS_EQ,
                arithmeticTheory.GREATER_EQ]);
+
+val type_vs_length = Q.store_thm ("type_vs_length",
+`∀tvs tenvC tenvS vs ts.
+  type_vs tvs tenvC tenvS vs ts ⇒ (LENGTH vs = LENGTH ts)`,
+induct_on `vs` >>
+rw [Once type_v_cases] >>
+rw [] >>
+metis_tac []);
+
+(* Typing lists of values from the end *)
+val type_vs_end = Q.store_thm ("type_vs_end",
+`∀tvs tenvC vs ts v t tenvS.
+  type_vs tvs tenvC tenvS (vs++[v]) (ts++[t]) =
+  (type_v tvs tenvC tenvS v t ∧
+   type_vs tvs tenvC tenvS vs ts)`,
+induct_on `vs` >>
+rw [] >>
+cases_on `ts` >>
+fs [] >>
+EQ_TAC >>
+rw [] >|
+[pop_assum (ASSUME_TAC o SIMP_RULE (srw_ss ()) [Once type_v_cases]) >>
+     fs [],
+ pop_assum (ASSUME_TAC o SIMP_RULE (srw_ss ()) [Once type_v_cases]) >>
+     fs [],
+ metis_tac [type_v_rules],
+ imp_res_tac type_vs_length >>
+     fs [],
+ imp_res_tac type_vs_length >>
+     fs [],
+ imp_res_tac type_vs_length >>
+     fs [],
+ imp_res_tac type_vs_length >>
+     fs [],
+ imp_res_tac type_vs_length >>
+     fs [],
+ imp_res_tac type_vs_length >>
+     fs [],
+ pop_assum (ASSUME_TAC o SIMP_RULE (srw_ss ()) [Once type_v_cases]) >>
+     fs [] >>
+     metis_tac [],
+ pop_assum (ASSUME_TAC o SIMP_RULE (srw_ss ()) [Once type_v_cases]) >>
+     fs [] >>
+     metis_tac [type_v_rules],
+ rw [Once type_v_cases] >>
+     pop_assum (ASSUME_TAC o SIMP_RULE (srw_ss ()) [Once type_v_cases]) >>
+     fs []]);
+
+(* Everything in the type environment is also in the execution environment *)
+val type_lookup_lem = Q.prove (
+`∀tenvC env tenvS tenv v n t' idx.
+  type_env tenvC tenvS env tenv ∧
+  (lookup_tenv n idx tenv = SOME t')
+  ⇒
+  (∃v'. lookup n env = SOME v')`,
+induct_on `tenv` >>
+rw [Once type_v_cases, lookup_def, bind_def] >>
+fs [lookup_tenv_def, bind_tenv_def] >-
+metis_tac [] >>
+every_case_tac >>
+fs [] >>
+metis_tac []);
+
+val type_lookup = Q.store_thm ("type_lookup",
+`∀tenvC env tenvS tenv v n t' idx tvs.
+  type_env tenvC tenvS env tenv ∧
+  (lookup_tenv n idx (bind_tvar tvs tenv) = SOME t')
+  ⇒
+  (∃v'. lookup n env = SOME v')`,
+induct_on `tvs` >>
+rw [bind_tvar_def] >-
+metis_tac [type_lookup_lem] >>
+fs [bind_tvar_def, lookup_tenv_def] >>
+rw [] >>
+every_case_tac >>
+fs [lookup_tenv_def] >>
+`!x y. x + SUC y = (x + 1) + y` by decide_tac >>
+metis_tac []);
+
+val type_lookup_id = Q.store_thm ("type_lookup_id",
+`∀tenvS tenvC menv tenvM (cenv : envC) tenv.
+  type_env tenvC tenvS env tenv ∧
+  consistent_mod_env tenvS tenvC menv tenvM 
+  ⇒
+  ((t_lookup_var_id n tenvM (bind_tvar tvs tenv) = SOME (tvs', t)) ⇒ 
+     (∃v. (lookup_var_id n (menv,cenv,env) = SOME v)))`,
+ induct_on `tenvM` >>
+ rw [t_lookup_var_id_def] >>
+ cases_on `n` >>
+ fs [] >>
+ rw [lookup_var_id_def, t_lookup_var_id_def] >>
+ imp_res_tac type_lookup
+ >- (Cases_on `v'` >>
+     fs [])
+ >- (Cases_on `v'` >>
+     fs [])
+ >- (qpat_assum `consistent_mod_env tenvS x0 x1 x2` (ASSUME_TAC o SIMP_RULE (srw_ss()) [Once type_v_cases]) >>
+     fs [] >>
+     rw [] >>
+     fs [t_lookup_var_id_def, lookup_var_id_def]
+     >- (match_mp_tac type_lookup >>
+         cases_on `lookup mn' tenvM` >>
+         fs [lookup_tenv_def, bind_tvar_def, bvl2_lookup] >>
+         metis_tac [])
+     >- metis_tac []));
+
+val type_subst = Q.store_thm ("type_subst",
+`(!tvs ctMap tenvS v t. type_v tvs ctMap tenvS v t ⇒
+    ∀targs tvs'.
+      (tvs = LENGTH targs) ∧
+      ctMap_ok ctMap ∧
+      EVERY (check_freevars tvs' []) targs ∧
+      check_freevars (LENGTH targs) [] t
+      ⇒
+      type_v tvs' ctMap tenvS v
+             (deBruijn_subst 0 targs (deBruijn_inc (LENGTH targs) tvs' t))) ∧
+ (!tvs ctMap tenvS vs ts. type_vs tvs ctMap tenvS vs ts ⇒
+   ∀targs tvs'.
+     (tvs = LENGTH targs) ∧
+     ctMap_ok ctMap ∧
+     EVERY (check_freevars tvs' []) targs ∧
+     EVERY (check_freevars (LENGTH targs) []) ts
+     ⇒
+     type_vs tvs' ctMap tenvS vs
+             (MAP (deBruijn_subst 0 targs) (MAP (deBruijn_inc (LENGTH targs) tvs') ts))) ∧
+ (!ctMap tenvS env tenv. type_env ctMap tenvS env tenv ⇒ 
+    type_env ctMap tenvS env tenv) ∧
+ (!ctMap tenvS envM tenvM. consistent_mod_env ctMap tenvS envM tenvM ⇒ 
+    consistent_mod_env ctMap tenvS envM tenvM)`,
+ ho_match_mp_tac type_v_strongind >>
+ rw [] >>
+ rw [Once type_v_cases] >>
+ pop_assum (ASSUME_TAC o SIMP_RULE (srw_ss()) [Once type_v_cases]) >>
+ rw [deBruijn_inc_def, deBruijn_subst_def] >>
+ rw [deBruijn_inc_def, deBruijn_subst_def] >>
+ fs [check_freevars_def, Tfn_def, Tint_def, Tbool_def, Tref_def, Tunit_def] >>
+ rw [deBruijn_inc_def, deBruijn_subst_def] >>
+ rw [nil_deBruijn_inc, deBruijn_subst_check_freevars, type_subst_lem3,
+     nil_deBruijn_subst]
+ >- (rw [EVERY_MAP] >>
+     fs [EVERY_MEM] >>
+     rw [] >>
+     metis_tac [type_subst_lem1, EVERY_MEM])
+ >- (`EVERY (check_freevars 0 tvs') ts` by metis_tac [ctMap_ok_lookup, EVERY_MEM] >>
+     `EVERY (check_freevars (LENGTH targs) tvs') ts`
+           by (`LENGTH targs ≥ 0` by decide_tac >>
+               metis_tac [EVERY_MEM, check_freevars_add]) >>
+     `type_vs tvs'' ctMap tenvS vs
+              (MAP (deBruijn_subst 0 targs)
+                 (MAP (deBruijn_inc (LENGTH targs) tvs'')
+                    (MAP (type_subst (ZIP (tvs',ts'))) ts)))`
+            by metis_tac [check_freevars_subst_list] >>
+     pop_assum mp_tac >>
+     rw [type_subst_deBruijn_subst_list, type_subst_deBruijn_inc_list] >>
+     metis_tac [])
+ >- metis_tac []
+ >- (qexists_tac `menv` >>
+     qexists_tac `tenvC` >>
+     qexists_tac `tenv` >>
+     rw [] >>
+     match_mp_tac type_e_subst_lem >>
+     rw [tenv_ok_def, bind_tvar_def] >>
+     metis_tac [type_v_freevars, ctMap_ok_lookup, consistent_con_env_def])
+ >- (qexists_tac `menv` >>
+     qexists_tac `tenvC` >>
+     qexists_tac `tenv` >>
+     qexists_tac `MAP (λ(x,t). (x,deBruijn_subst 0 targs t)) tenv'` >>
+     rw [] >|
+     [match_mp_tac type_funs_subst_lem >>
+          rw [] >-
+          metis_tac [type_v_freevars] >-
+          metis_tac [consistent_con_env_def] >>
+          match_mp_tac tenv_ok_bind_var_list_funs >>
+          metis_tac [tenv_ok_bind_var_list_funs, type_v_freevars, bind_tvar_rewrites],
+      qpat_assum `type_funs w0 w x y z` (fn x => ALL_TAC) >>
+          induct_on `tenv'` >>
+          fs [lookup_def] >>
+          rw [] >>
+          PairCases_on `h` >>
+          fs [] >>
+          rw [] >>
+          metis_tac []])
+ >- (fs [bind_def, bind_tenv_def] >>
+     metis_tac [type_v_rules])
+ >- (fs [bind_def, bind_tenv_def] >>
+     rw [Once type_v_cases, bind_def, bind_tenv_def]));
+
+(* They value of a binding in the execution environment has the type given by
+ * the type environment. *)
+val type_lookup_lem2 = Q.prove (
+`∀ctMap env tenv tvs tenvS v x t targs tparams idx.
+  ctMap_ok ctMap ∧
+  type_env ctMap tenvS env tenv ∧
+  EVERY (check_freevars tvs []) targs ∧
+  (lookup_tenv x 0 (bind_tvar tvs tenv) = SOME (LENGTH targs, t)) ∧
+  (lookup x env = SOME v)
+  ⇒
+  type_v tvs ctMap tenvS v (deBruijn_subst 0 targs t)`,
+induct_on `tenv` >>
+rw [] >>
+fs [lookup_tenv_def, bind_tvar_def] >>
+qpat_assum `type_env ctMap tenvS env tenv_pat`
+        (MP_TAC o SIMP_RULE (srw_ss ())
+                         [Once type_env_cases]) >>
+rw [] >>
+fs [lookup_def, bind_def, emp_def, bind_tenv_def] >>
+rw [] >>
+cases_on `n'≠x` >>
+rw [] >-
+metis_tac [lookup_tenv_def] >>
+`(n = LENGTH targs) ∧ (t = deBruijn_inc n tvs t')`
+          by (cases_on `tvs` >>
+              fs [lookup_tenv_def] >>
+              metis_tac []) >>
+rw [] >>
+metis_tac [type_v_freevars, type_subst, bind_tvar_def]);
+
+val consistent_mod_env_lookup = Q.prove (
+`!tenvS ctMap menv tenvM tenv env n.
+  consistent_mod_env tenvS ctMap menv tenvM ∧
+  (lookup n menv = SOME env) ∧
+  (lookup n tenvM = SOME tenv)
+  ⇒
+  type_env ctMap tenvS env (bind_var_list2 tenv Empty)`,
+induct_on `tenvM` >>
+rw [] >>
+cases_on `menv` >>
+fs [] >>
+qpat_assum `consistent_mod_env x0 x1 x2 x3` (ASSUME_TAC o SIMP_RULE (srw_ss()) [Once consistent_mod_cases]) >>
+fs [] >>
+rw [] >>
+fs [] >>
+every_case_tac >>
+fs [] >>
+metis_tac []);
+
+val type_lookup_type_v = Q.store_thm ("type_lookup_type_v",
+`∀tenvM ctMap menv env tenv tvs tenvS v x t targs tparams idx.
+  tenvM_ok tenvM ∧
+  ctMap_ok ctMap ∧
+  type_env ctMap tenvS env tenv ∧
+  consistent_mod_env tenvS ctMap menv tenvM ∧
+  EVERY (check_freevars tvs []) targs ∧
+  (t_lookup_var_id x tenvM (bind_tvar tvs tenv) = SOME (LENGTH targs, t)) ∧
+  (lookup_var_id x (menv,cenv,env) = SOME v)
+  ⇒
+  type_v tvs ctMap tenvS v (deBruijn_subst 0 targs t)`,
+ cases_on `x` >>
+ rw [] >>
+ fs [lookup_var_id_def, t_lookup_var_id_def] >-
+ metis_tac [type_lookup_lem2] >>
+ every_case_tac >>
+ fs [] >>
+ match_mp_tac type_lookup_lem2 >>
+ rw [bind_tvar_rewrites] >>
+ imp_res_tac consistent_mod_env_lookup >>
+ qexists_tac `x` >>
+ qexists_tac `bind_var_list2 x' Empty` >>
+ qexists_tac `a` >>
+ rw [] >>
+ metis_tac [tenvM_ok_lookup, type_lookup_lem4, num_tvs_bvl2, num_tvs_def, bvl2_lookup]);
+
+val type_env_merge_bvl2 = Q.store_thm ("type_env_merge_bvl2",
+`!tenvM tenvC tenvS env1 tenv1 env2 tenv2.
+  type_env tenvC tenvS env2 (bind_var_list2 tenv2 Empty) ∧
+  type_env tenvC tenvS env1 (bind_var_list2 tenv1 Empty) ⇒
+  type_env tenvC tenvS (merge env1 env2) (bind_var_list2 (tenv1 ++ tenv2) Empty)`,
+induct_on `env1` >>
+cases_on `tenv1` >>
+rw [merge_def] >>
+rw [Once type_v_cases] >>
+rw [emp_def, bind_def] >>
+PairCases_on `h` >>
+fs [bind_var_list2_def, bind_tenv_def] >>
+pop_assum (ASSUME_TAC o SIMP_RULE (srw_ss()) [Once type_v_cases]) >>
+fs [bind_def, emp_def, bind_tenv_def] >>
+metis_tac [merge_def]);
 
 (* ---------- constructor checking stuff ---------- *)
 (* check_new_type, check_ctor_tenv, build_ctor_tenv, check_new_exn,
@@ -2006,6 +2416,123 @@ val extend_consistent_con_exn = Q.store_thm ("extend_consistent_con_exn",
  every_case_tac >>
  fs [FLOOKUP_DEF]);
 
+val consistent_con_env_lookup = Q.store_thm ("consistent_con_env_lookup",
+`!ctMap envC tenvC cn tvs ts tn.
+  consistent_con_env ctMap envC tenvC ∧
+  lookup_con_id cn tenvC = SOME (tvs,ts,tn)
+  ⇒
+  FLOOKUP ctMap (id_to_n cn,tn) = SOME (tvs, ts)`,
+ rw [consistent_con_env_def] >>
+ cases_on `lookup_con_id cn envC` >>
+ fs [] >>
+ res_tac >>
+ fs [] >>
+ PairCases_on `x` >>
+ res_tac >>
+ fs [] >>
+ rw []);
+
+val consistent_con_env_to_mod = Q.store_thm ("consistent_con_env_to_mod",
+`!ctMap envC flat_envC tenvC flat_tenvC mn.
+  MAP FST flat_envC = MAP FST flat_tenvC ∧
+  consistent_con_env ctMap envC tenvC ∧
+  consistent_con_env ctMap (merge_envC (emp,flat_envC) envC) (merge_tenvC (emp,flat_tenvC) tenvC)
+  ⇒
+  consistent_con_env ctMap (merge_envC ([(mn,flat_envC)],emp) envC) (merge_tenvC ([(mn,flat_tenvC)],emp) tenvC)`,
+ rw [consistent_con_env_def] >>
+ PairCases_on `tenvC` >>
+ PairCases_on `envC` >>
+ fs [merge_envC_def, merge_tenvC_def, merge_def, emp_def]
+ >- fs [tenvC_ok_def, flat_tenvC_ok_def]
+ >- (`(?mn' cn'. cn = Long mn' cn') ∨ (?cn'. cn = Short cn')` by (Cases_on `cn` >> metis_tac []) >>
+     fs [lookup_con_id_mod_cons] >>
+     rw []
+     >- (FIRST_X_ASSUM (mp_tac o Q.SPECL [`Short cn'`, `n`, `t`]) >>
+         fs [lookup_con_id_def] >>
+         rw [] >>
+         fs [lookup_append] >>
+         every_case_tac >>
+         fs [] >>
+         rw [] >>
+         fs [id_to_n_def] >>
+         imp_res_tac lookup_in2 >>
+         fs [MEM_MAP, lookup_notin] >>
+         metis_tac [MEM_MAP])
+     >- (fs [] >>
+         FIRST_X_ASSUM (mp_tac o Q.SPECL [`Long mn' cn'`, `n`, `t`]) >>
+         fs [lookup_con_id_def] >>
+         rw [])
+     >- (LAST_X_ASSUM (mp_tac o Q.SPECL [`Short cn'`, `n`, `t`]) >>
+         fs [lookup_con_id_def] >>
+         rw []))
+ >- (`(?mn' cn'. cn = Long mn' cn') ∨ (?cn'. cn = Short cn')` by (Cases_on `cn` >> metis_tac []) >>
+     fs [lookup_con_id_mod_cons] >>
+     rw [] >>
+     fs [lookup_notin]
+     >- metis_tac []
+     >- (rpt (LAST_X_ASSUM (mp_tac o Q.SPECL [`Short cn'`])) >>
+         fs [lookup_con_id_def] >>
+         rw [])));
+
+(* ---------- type_ctxt, type_ctxts ---------- *)
+
+val type_ctxts_freevars = Q.store_thm ("type_ctxts_freevars",
+`!tvs ctMap tenvS cs t1 t2.
+  type_ctxts tvs ctMap tenvS cs t1 t2 ⇒
+  ctMap_ok ctMap ⇒
+  check_freevars tvs [] t1 ∧ check_freevars tvs [] t2`,
+ ho_match_mp_tac type_ctxts_ind >>
+ rw [type_ctxt_cases, check_freevars_def, Tbool_def] >>
+ rw [check_freevars_def] 
+ >- rw [Texn_def, check_freevars_def]
+ >- (cases_on `pes` >>
+     fs [RES_FORALL] >>
+     qpat_assum `!x. (x = h) ∨ MEM x t ⇒ P x` (ASSUME_TAC o Q.SPEC `h`) >>
+     fs [] >>
+     PairCases_on `h` >>
+     fs [] >>
+     fs [Once context_invariant_cases] >>
+     metis_tac [type_p_freevars])
+ >- (imp_res_tac ctMap_ok_lookup >>
+     fs [] >>
+     match_mp_tac check_freevars_subst_single >>
+     rw [] >>
+     imp_res_tac consistent_con_env_lookup >>
+     res_tac >>
+     fs [] >>
+     metis_tac [check_freevars_add, arithmeticTheory.ZERO_LESS_EQ,
+                arithmeticTheory.GREATER_EQ])
+ >- rw [Texn_def, check_freevars_def]
+ >- metis_tac [check_freevars_add, arithmeticTheory.ZERO_LESS_EQ, arithmeticTheory.GREATER_EQ]
+ >- metis_tac [check_freevars_add, arithmeticTheory.ZERO_LESS_EQ, arithmeticTheory.GREATER_EQ]
+ >- metis_tac [check_freevars_add, arithmeticTheory.ZERO_LESS_EQ, arithmeticTheory.GREATER_EQ]
+ >- metis_tac [check_freevars_add, arithmeticTheory.ZERO_LESS_EQ, arithmeticTheory.GREATER_EQ]
+ >- metis_tac [check_freevars_add, arithmeticTheory.ZERO_LESS_EQ, arithmeticTheory.GREATER_EQ]
+ >- metis_tac [check_freevars_add, arithmeticTheory.ZERO_LESS_EQ, arithmeticTheory.GREATER_EQ]
+ >- metis_tac [check_freevars_add, arithmeticTheory.ZERO_LESS_EQ, arithmeticTheory.GREATER_EQ]
+ >- metis_tac [check_freevars_add, arithmeticTheory.ZERO_LESS_EQ, arithmeticTheory.GREATER_EQ]
+ >- (cases_on `pes` >>
+     fs [RES_FORALL] >>
+     qpat_assum `!x. (x = h) ∨ MEM x t ⇒ P x` (ASSUME_TAC o Q.SPEC `h`) >>
+     fs [] >>
+     PairCases_on `h` >>
+     fs [] >>
+     fs [Once context_invariant_cases] >>
+     metis_tac [type_p_freevars])
+ >- metis_tac [check_freevars_add, arithmeticTheory.ZERO_LESS_EQ, arithmeticTheory.GREATER_EQ]
+ >- metis_tac [check_freevars_add, arithmeticTheory.ZERO_LESS_EQ, arithmeticTheory.GREATER_EQ]
+ >- (imp_res_tac ctMap_ok_lookup >>
+     fs [] >>
+     match_mp_tac check_freevars_subst_single >>
+     rw [] >>
+     imp_res_tac consistent_con_env_lookup >>
+     res_tac >>
+     fs [] >>
+     metis_tac [check_freevars_add, arithmeticTheory.ZERO_LESS_EQ,
+                arithmeticTheory.GREATER_EQ])
+ >- metis_tac [check_freevars_add, arithmeticTheory.ZERO_LESS_EQ, arithmeticTheory.GREATER_EQ]
+ >- metis_tac [check_freevars_add, arithmeticTheory.ZERO_LESS_EQ, arithmeticTheory.GREATER_EQ]);
+
 (* ---------- type_d ---------- *)
 
 val type_d_tenv_ok = Q.store_thm ("type_d_tenv_ok",
@@ -2050,6 +2577,44 @@ val type_d_ctMap_ok = Q.store_thm ("type_d_ctMap_ok",
  >- (imp_res_tac check_exn_tenv_disjoint >>
      fs [FDOM_FUPDATE_LIST, flat_to_ctMap_def, flat_to_ctMap_list_def] >>
      metis_tac [emp_def,DISJOINT_SYM]));
+
+val ctMap_ok_pres = Q.store_thm ("ctMap_ok_pres",
+`!mn tenvM tenvC tenv d tenvC' tenv'.
+  type_d mn tenvM tenvC tenv d tenvC' tenv' ∧
+  ctMap_ok (to_ctMap tenvC)
+  ⇒
+  ctMap_ok (FUNION (flat_to_ctMap tenvC') (to_ctMap tenvC)) ∧
+  DISJOINT (FDOM (flat_to_ctMap tenvC')) (FDOM (to_ctMap tenvC))`,
+ rw [] >>
+ imp_res_tac type_d_ctMap_ok >>
+ rw [] >>
+ rw [GSYM merge_def] >>
+ imp_res_tac ctMap_ok_merge_imp >>
+ rw [] >>
+ metis_tac [DISJOINT_SYM]);
+
+val type_d_mod = Q.store_thm ("type_d_mod",
+`!mn tenvM tenvC tenv d tenvC' tenv'.
+  type_d mn tenvM tenvC tenv d tenvC' tenv'
+  ⇒
+  ctMap_to_mods (flat_to_ctMap tenvC') ⊆ { mn }`,
+ rw [type_d_cases, ctMap_to_mods_def, emp_def, SUBSET_DEF, bind_def, flat_to_ctMap_def,
+     flat_to_ctMap_list_def, FDOM_FUPDATE_LIST] >>
+ fs [build_ctor_tenv_def, MEM_FLAT, MEM_MAP] >>
+ rw [] >>
+ TRY (PairCases_on `y''''`) >>
+ TRY (PairCases_on `y'''''`) >>
+ fs [MEM_MAP] >>
+ rw [] >>
+ TRY (PairCases_on `y'`) >>
+ TRY (PairCases_on `y''`) >>
+ fs [mk_id_def] >>
+ rw [] >>
+ every_case_tac >>
+ fs [MEM_MAP] >>
+ TRY (PairCases_on `y`) >>
+ TRY (PairCases_on `y'`) >>
+ fs []);
 
 (* ---------- type_ds ---------- *)
 
@@ -2103,6 +2668,20 @@ val type_ds_ctMap_ok = Q.store_thm ("type_ds_ctMap_ok",
          to_ctMap_list_def, MEM_FLAT, flat_to_ctMap_list_append, merge_def] >>
      metis_tac []));
 
+val type_ds_mod = Q.store_thm ("type_ds_mod",
+`!mn tenvM tenvC tenv ds tenvC' tenv'.
+  type_ds mn tenvM tenvC tenv ds tenvC' tenv'
+  ⇒
+  ctMap_to_mods (flat_to_ctMap tenvC') ⊆ { mn }`,
+ induct_on `ds` >>
+ rw [Once type_ds_cases]
+ >- rw [emp_def, ctMap_to_mods_def, SUBSET_DEF, flat_to_ctMap_def, FDOM_FUPDATE_LIST,
+        MEM_MAP, flat_to_ctMap_list_def] >>
+ imp_res_tac type_d_mod >>
+ rw [ctMap_to_mods_append, merge_def, flat_to_ctMap_append] >>
+ metis_tac []);
+
+
 (* ---------- type_specs ---------- *)
 
 val type_specs_tenv_ok = Q.store_thm ("type_specs_tenv_ok",
@@ -2120,5 +2699,36 @@ rw [rich_listTheory.LENGTH_COUNT_LIST, EVERY_MAP] >>
 rw [EVERY_MEM] >>
 fs [rich_listTheory.MEM_COUNT_LIST, check_freevars_def] >>
 metis_tac [check_freevars_add, DECIDE ``!x:num. x ≥ 0``]);
+
+val type_specs_mod = Q.store_thm ("type_specs_mod",
+`!mn tenvC tenv specs tenvC' tenv'.
+  type_specs mn tenvC tenv specs tenvC' tenv'
+  ⇒
+  !mn'. mn = SOME mn' ⇒
+  ctMap_to_mods (flat_to_ctMap tenvC) ⊆ {mn}
+  ⇒
+  ctMap_to_mods (flat_to_ctMap tenvC') ⊆ {mn}`,
+ ho_match_mp_tac type_specs_ind >>
+ rw [] >>
+ FIRST_X_ASSUM match_mp_tac >>
+ rw [] >>
+ fs [merge_def, flat_to_ctMap_append, ctMap_to_mods_append, bind_def] >>
+ SIMP_TAC (bool_ss) [Once (METIS_PROVE [APPEND] ``x::y = [x]++y``), flat_to_ctMap_append, ctMap_to_mods_append] >>
+ rw [] >>
+ rpt (pop_assum (fn _ => all_tac)) >>
+ rw [build_ctor_tenv_def, MEM_FLAT, MEM_MAP, ctMap_to_mods_def, SUBSET_DEF,
+     flat_to_ctMap_def, FDOM_FUPDATE_LIST, flat_to_ctMap_list_def] >>
+ TRY (PairCases_on `y'`) >>
+ TRY (PairCases_on `y''`) >>
+ TRY (PairCases_on `y'''`) >>
+ TRY (PairCases_on `y''''`) >>
+ fs [MEM_MAP] >>
+ rw [] >>
+ TRY (PairCases_on `y`) >>
+ TRY (PairCases_on `y'`) >>
+ fs [bind_def, mk_id_def] >>
+ rw [] >>
+ every_case_tac >>
+ fs []);
 
 val _ = export_theory ();
